Alg/ListProps/Sorted/Union.lean
@@ -52,68 +52,68 @@ theorem List.sorted_union.induct_gt [Compare α] : ∀{a b: α} {as bs: List α}
 
 #print axioms List.sorted_union.induct_gt
 
-def List.sorted_union.sublist_of_left [Compare α] : ∀{as bs: List α},
-  as.sublist_of (as.sorted_union bs) := by
+def List.sorted_union.subset_of_left [Compare α] : ∀{as bs: List α},
+  as.subset_of (as.sorted_union bs) := by
   apply sorted.induction
   {
     intro bs
     rw [empty_left]
-    exact List.sublist_of.empty
+    exact List.subset_of.empty
   }
   {
     intro a as
     rw [empty_right]
-    exact List.sublist_of.id
+    exact List.subset_of.id
   }
   {
     intro a as b bs a_ord_b prev
     rw [induct_lt a_ord_b]
-    apply List.sublist_of.push
+    apply List.subset_of.push
     assumption
   }
   {
     intro a as b bs a_ord_b prev
     rw [induct_eq a_ord_b]
-    apply List.sublist_of.push
+    apply List.subset_of.push
     assumption
   }
   {
     intro a as b bs a_ord_b prev
     rw [induct_gt a_ord_b]
-    apply List.sublist_of.push_right
+    apply List.subset_of.push_right
     assumption
   }
 
-def List.sorted_union.sublist_of_right [Compare α] : ∀{as bs: List α},
-  bs.sublist_of (as.sorted_union bs) := by
+def List.sorted_union.subset_of_right [Compare α] : ∀{as bs: List α},
+  bs.subset_of (as.sorted_union bs) := by
   apply sorted.induction
   {
     intro bs
     rw [empty_left]
-    exact List.sublist_of.id
+    exact List.subset_of.id
   }
   {
     intro a as
     rw [empty_right]
-    exact List.sublist_of.empty
+    exact List.subset_of.empty
   }
   {
     intro a as b bs a_ord_b prev
     rw [induct_lt a_ord_b]
-    apply List.sublist_of.push_right
+    apply List.subset_of.push_right
     assumption
   }
   {
     intro a as b bs a_ord_b prev
     rw [induct_eq a_ord_b]
     rw [Compare.ord_to_eq a_ord_b]
-    apply List.sublist_of.push
+    apply List.subset_of.push
     assumption
   }
   {
     intro a as b bs a_ord_b prev
     rw [induct_gt a_ord_b]
-    apply List.sublist_of.push
+    apply List.subset_of.push
     assumption
   }
 
