Alg/ListProps/Sorted/Merge.lean
@@ -299,16 +299,16 @@ def List.sorted_merge.contains [Compare α] (as bs: List α) (x: α) : as.contai
 
 #print axioms List.sorted_merge.contains
 
-def List.sorted_merge.src_left_sublist [Compare α] {as bs: List α} :
-  as.sublist_of (as.sorted_merge bs) := by
+def List.sorted_merge.src_left_subset [Compare α] {as bs: List α} :
+  as.subset_of (as.sorted_merge bs) := by
   intro x con
   exact List.sorted_merge.contains as bs x (Or.inl con)
 
-#print axioms List.sorted_merge.src_left_sublist
+#print axioms List.sorted_merge.src_left_subset
 
-def List.sorted_merge.src_right_sublist [Compare α] {as bs: List α} :
-  bs.sublist_of (as.sorted_merge bs) := by
+def List.sorted_merge.src_right_subset [Compare α] {as bs: List α} :
+  bs.subset_of (as.sorted_merge bs) := by
   intro x con
   exact List.sorted_merge.contains as bs x (Or.inr con)
 
-#print axioms List.sorted_merge.src_right_sublist
+#print axioms List.sorted_merge.src_right_subset
